lib/Buckets/PackedKV.i.dfy
@@ -60,12 +60,71 @@ module PackedKV {
     )
   }
 
+  predicate EncodableMessage(msg: Message)
+  {
+    && msg.Define?
+  }
+
+  predicate EncodableMessageSeq(msgs: seq<Message>)
+  {
+    && (forall i | 0 <= i < |msgs| :: EncodableMessage(msgs[i]))
+  }
+
   function method Message_to_bytestring(msg: Message) : seq<byte>
     requires msg.Define?
   {
     msg.value
   }
   
+  function messageSeq_to_bytestringSeq(msgs: seq<Message>) : (result: seq<seq<byte>>)
+    requires EncodableMessageSeq(msgs)
+    ensures |result| == |msgs|
+    ensures forall i | 0 <= i < |result| :: result[i] == Message_to_bytestring(msgs[i])
+  {
+    if |msgs| == 0 then
+      []
+    else
+      messageSeq_to_bytestringSeq(Sequences.DropLast(msgs)) + [ Message_to_bytestring(Last(msgs)) ]
+  }
+
+  function bytestringSeq_to_MessageSeq(strings: seq<seq<byte>>) : (result: seq<Message>)
+    requires forall i | 0 <= i < |strings| :: |strings[i]| < 0x1_0000_0000
+    ensures |result| == |strings|
+    ensures forall i | 0 <= i < |strings| :: result[i] == bytestring_to_Message(strings[i])
+  {
+    if |strings| == 0 then
+      []
+    else
+      bytestringSeq_to_MessageSeq(Sequences.DropLast(strings)) + [ bytestring_to_Message(Last(strings)) ]
+  }
+
+  lemma messageSeq_to_bytestringSeq_Additive(msgs1: seq<Message>, msgs2: seq<Message>)
+    requires EncodableMessageSeq(msgs1)
+    requires EncodableMessageSeq(msgs2)
+    ensures EncodableMessageSeq(msgs1 + msgs2)
+    ensures messageSeq_to_bytestringSeq(msgs1 + msgs2) == messageSeq_to_bytestringSeq(msgs1) + messageSeq_to_bytestringSeq(msgs2)
+  {
+  }
+  
+  method MessageArray_to_bytestringSeq(msgs: array<Message>, nmsgs: uint64) returns (result: seq<seq<byte>>)
+    requires nmsgs as nat <= msgs.Length
+    requires EncodableMessageSeq(msgs[..nmsgs])
+    ensures result[..] == messageSeq_to_bytestringSeq(msgs[..nmsgs])
+  {
+    var aresult := new seq<byte>[nmsgs];
+    var i: uint64 := 0;
+
+    while i < nmsgs
+      invariant i <= nmsgs
+      invariant aresult[..i] == messageSeq_to_bytestringSeq(msgs[..i])
+    {
+      aresult[i] := Message_to_bytestring(msgs[i]);
+      i := i + 1;
+    }
+
+    result := aresult[..i];
+  }
+
   function IKeys(psa: PSA.Psa) : (res : seq<Key>)
   requires PSA.WF(psa)
   requires ValidStringLens(PSA.I(psa), KeyType.MaxLen() as nat)
